Finalizacao

escrow.bpl
@@ -2,10 +2,9 @@ type Ref;
 type string; //declarando um tipo string
 type bytes20;
 type bytes32;
-type uint8;
-type uint32;
-type uint256;
 type Field G; 
+
+//type x = int where 0 < x ;
 
 type address; 
 const unique zeroAddress: address;
@@ -21,18 +20,18 @@ const unique TOKEN: TransactionType;
 
 type Transaction = <G>[Ref, Field G] G;
 const null : Transaction; //Declarando um tipo null para referencias.. 
-var value : Field uint256;
-var lastModified : Field uint256;
+var value : Field int;
+var lastModified : Field int;
 var status : Field Status;
 var transactionType : Field TransactionType;
-var threshold : Field uint8;
-var timeoutHours : Field uint32;
+var threshold : Field int;
+var timeoutHours : Field int;
 var buyer : Field address;
 var seller : Field address;
 var tokenAddress : Field address; 
 var moderator : Field address;
-var released : Field uint256;
-var noOfReleases : Field uint256; 
+var released : Field int;
+var noOfReleases : Field int; 
 var isOwner : Field [address] bool;
 var voted : Field [bytes32] bool;
 var beneficiaries : Field [address] bool;
@@ -49,37 +48,81 @@ var transactionCount : int;
 
 //-----------------------------Modifiers--------------------------------------------
 
- function transactionDoesNotExistModifier(scriptHash : bytes32) returns (bool) {
-    Transactions[scriptHash] == null;
-    //var transaction : Transaction;
-    //transaction := Transactions[scriptHash];
-    //transactionExists := transaction == null;
-    }
+ function transactionDoesNotExistModifier(scriptHash : bytes32, this : Ref, transactionsMap : [bytes32] Transaction) returns (bool) {
+    (transactionsMap[scriptHash] == null)
+}
 
+function transactionExistsModifier(scriptHash : bytes32, this : Ref, transactionsMap : [bytes32] Transaction) returns (bool) {
+    (transactionsMap[scriptHash] != null)
+}
+
+function inFundedStateModifier(scriptHash : bytes32) returns (bool) {
+       true
+}
+
+function fundsExistModifier(scriptHash : bytes32) returns (bool) {
+    true
+}
+
+function nonZeroAddressModifier(addressToCheck : address) returns (bool) {
+    true
+}
+
+function checkTransactionTypeModifier(scriptHash : bytes32, transactionType : TransactionType) returns (bool) {
+    true
+}
+
+function onlyBuyerModifier(scriptHash : bytes32) returns (bool) {
+    true
+}
 
 //-------------------------------------------------------------------------
 
 
-procedure addTransaction(buyer : address, seller : address, moderator : address, threshold : uint8, 
-timeoutHours : uint32, scriptHash: bytes32, uniqueId : bytes20, msg.sender : address, msg.value : uint256 ) 
-requires transactionDoesNotExistModifier(scriptHash); {
+procedure addTransaction(buyer : address, seller : address, moderator : address, threshold : int, 
+timeoutHours : int, scriptHash: bytes32, uniqueId : bytes20, msg.sender : address, msg.value : int, this : Ref )
+requires transactionDoesNotExistModifier(scriptHash, this, Transactions); 
+requires nonZeroAddressModifier(buyer);
+requires nonZeroAddressModifier(seller);{
 
+    
     call addTransaction_ (buyer, seller, moderator, threshold, timeoutHours, scriptHash, msg.value, 
     uniqueId, ETHER, zeroAddress, msg.sender);
 }
 
-procedure addTokenTransaction(buyer : address, seller : address, moderator : address, threshold : uint8, 
-timeoutHours : uint32, scriptHash: bytes32, value : uint256, uniqueId : bytes20, msg.sender : address ) {
+procedure addTokenTransaction(buyer : address, seller : address, moderator : address, threshold : int, 
+timeoutHours : int, scriptHash: bytes32, value : int, uniqueId : bytes20, msg.sender : address ) {
 
     call addTransaction_ (buyer, seller, moderator, threshold, timeoutHours, scriptHash, value, 
     uniqueId, TOKEN, zeroAddress, msg.sender);
 }
 
-procedure addTransaction_ (buyer : address, seller : address, moderator : address, threshold : uint8,
-timeoutHours : uint32, scriptHash : bytes32, value : uint256, uniqueId : bytes20, 
-transactionType : TransactionType, tokenAddress : address,  msg.sender : address) {
 
+
+procedure addTransaction_ (buyer : address, seller : address, moderator : address, threshold : int,
+timeoutHours : int, scriptHash : bytes32, value : int, uniqueId : bytes20, 
+transactionType : TransactionType, tokenAddress : address,  msg.sender : address) {
+   
+   var this : Ref;
+   var newTransaction : Transaction;
+   
+   assume (buyer != seller);
+   assume (value > 0);
+   assume (threshold > 0);
+   assume (threshold <= 3);
+   assume (threshold == 1 || moderator != zeroAddress);
+   assume (scriptHash == calculateRedeemScriptHash(uniqueId,threshold,timeoutHours, buyer, seller, moderator, tokenAddress ));
+
+  newTransaction[this, buyer] := Field buyer;
+
+    
 }
+
+function calculateRedeemScriptHash(uniqueId : bytes20, threshold : int, timeoutHours : int, buyer : address,
+seller : address, moderator : address, tokenAddress : address) returns (bytes32);
+    
+
+
 
 procedure checkBeneficiary(scriptHash : bytes32, beneficiary: address) {
 
@@ -89,7 +132,7 @@ procedure checkVote(scriptHash : bytes32, party : address) {
 
 }
 
-procedure addFundsToTransaction(scriptHash : bytes32, msg.value : uint256) {
+procedure addFundsToTransaction(scriptHash : bytes32, msg.value : int) {
 
 }
 
@@ -98,17 +141,13 @@ procedure getAllTransactionsForParty (partyAddress : address){
 }
 
 
-procedure execute( calldataSigV : [int] uint8, calldataSigR : [int] bytes32, calldataSigS : [int] bytes32,
-scriptHash : bytes32,  calldataDestinations : [int] address, calldataAmounts : [int] uint256) {
+procedure execute( calldataSigV : [int] int, calldataSigR : [int] bytes32, calldataSigS : [int] bytes32,
+scriptHash : bytes32,  calldataDestinations : [int] address, calldataAmounts : [int] int) {
 
 }
 
 procedure getTransactionHash(scriptHash : bytes32,  destinations : [int] address,
-amounts : [int] uint256) {
+amounts : [int] int) {
 
 }
 
-procedure calculateRedeemScriptHash(uniqueId : bytes20, threshold : uint8, timeoutHours : uint32,
-buyer : address, seller : address, moderator : address, tokenAddress : address ) {
-
-}
